\documentclass[12pt]{article}
\usepackage{amsmath}

\begin{document}

\begin{eqnarray*}
(a+b)^k & = & \sum_{i=0}^k \binom{k}{i}a^{i}b^{k-i} \\
  & = & a^k + \sum_{i=0}^{k-1} \binom{k}{i}a^{i}b^{k-i} \\
  & = & a^k + \sum_{i=0}^{k-1} \left(\binom{k-1}{i}+\binom{k-1}{i-1}\right)a^{i}b^{k-i} \\
  & = & a^k + \sum_{i=0}^{k-1} \binom{k-1}{i}a^{i}b^{k-i} 
	+\sum_{i=0}^{k-1}\binom{k-1}{i-1}a^{i}b^{k-i} \\
  & = & a^k + b\sum_{i=0}^{k-1} \binom{k-1}{i}a^{i}b^{(k-1)-i} 
	+ b\sum_{i=0}^{k-1}\binom{k-1}{i-1}a^{i}b^{(k-1)-i} \\
  & = & a^k + b(a+b)^{k-1}
	+ b\sum_{i=0}^{k-1}\binom{k-1}{i-1}a^{i}b^{(k-1)-i} \\
  & = & a^k + b(a+b)^{k-1}
	+ ab^2\sum_{i=0}^{k-1}\binom{k-1}{i-1}a^{i-1}b^{(k-2)-i} \\
  & = & a^k + b(a+b)^{k-1}
	+ ab^2\sum_{i=1}^{k-1}\binom{k-1}{i-1}a^{i-1}b^{(k-2)-i} \\
  & = & a^k + b(a+b)^{k-1}
	+ ab^2\sum_{i=0}^{k-2}\binom{k-1}{i}a^{i}b^{(k-1)-i} \\
  & = & a^k + b(a+b)^{k-1}
	+ ab^2\left(\sum_{i=0}^{k-1}\binom{k-1}{i}a^{i}b^{(k-1)-i} 
		- a^{k-1}\right) \\
  & = & a^k + b(a+b)^{k-1}
	+ ab^2((a+b)^{k-1} - a^{k-1}) \\
 & \le & a^k + 
	+ (b + ab^2)(a+b)^{k-1} \\
\end{eqnarray*}



\end{document}



